disk-betree/IndirectionTableImpl.i.dfy
@@ -1,0 +1,369 @@
+include "../lib/Maps.s.dfy"
+include "../lib/sequences.s.dfy"
+include "../lib/Option.s.dfy"
+include "../lib/NativeTypes.s.dfy"
+include "../lib/LRU.i.dfy"
+include "../lib/MutableMapModel.i.dfy"
+include "../lib/MutableMapImpl.i.dfy"
+include "PivotBetreeSpec.i.dfy"
+include "AsyncSectorDiskModel.i.dfy"
+include "BlockCacheSystem.i.dfy"
+include "../lib/Marshalling/GenericMarshalling.i.dfy"
+include "../lib/Bitmap.i.dfy"
+include "IndirectionTableModel.i.dfy"
+
+module IndirectionTableImpl {
+  import opened Maps
+  import opened Sets
+  import opened Options
+  import opened Sequences
+  import opened NativeTypes
+  import ReferenceType`Internal
+  import BT = PivotBetreeSpec`Internal
+  import BC = BetreeGraphBlockCache
+  import LruModel
+  import MutableMapModel
+  import MutableMap
+  import LBAType
+  import opened GenericMarshalling
+  import Bitmap
+  import opened Bounds
+  import IndirectionTableModel
+
+  type HashMap = MutableMap.ResizingHashMap<IndirectionTableModel.Entry>
+
+  // TODO move bitmap in here?
+  class IndirectionTable {
+    var t: HashMap;
+    ghost var Repr: set<object>;
+
+    protected predicate Inv()
+    reads this, Repr
+    ensures Inv() ==> this in Repr
+    {
+      && this in Repr
+      && this.t in Repr
+      && Repr == {this} + this.t.Repr
+      && this !in this.t.Repr
+      && t.Inv()
+    }
+
+    protected function I() : IndirectionTableModel.IndirectionTable
+    reads this, Repr
+    requires Inv()
+    ensures IndirectionTableModel.Inv(I())
+    {
+      IndirectionTableModel.FromHashMap(t.I())
+    }
+
+    method GetEntry(ref: BT.G.Reference) returns (e : Option<IndirectionTableModel.Entry>)
+    requires Inv()
+    ensures e == IndirectionTableModel.GetEntry(I(), ref)
+    {
+      IndirectionTableModel.reveal_GetEntry();
+      e := this.t.Get(ref);
+    }
+
+    method HasEmptyLoc(ref: BT.G.Reference) returns (b: bool)
+    requires Inv()
+    ensures b == IndirectionTableModel.HasEmptyLoc(I(), ref)
+    {
+      var entry := this.t.Get(ref);
+      b := entry.Some? && entry.value.loc.None?;
+    }
+
+    method RemoveLocIfPresent(ref: BT.G.Reference)
+    requires Inv()
+    modifies Repr
+    ensures Inv()
+    ensures forall o | o in Repr :: fresh(o) || o in old(Repr)
+    ensures I() == IndirectionTableModel.RemoveLocIfPresent(old(I()), ref)
+    {
+      IndirectionTableModel.reveal_RemoveLocIfPresent();
+
+      assume this.t.Count as nat < 0x10000000000000000 / 8;
+      var oldEntry := this.t.Get(ref);
+      if oldEntry.Some? {
+        this.t.Insert(ref, IndirectionTableModel.Entry(None, oldEntry.value.succs));
+      }
+
+      Repr := {this} + this.t.Repr;
+    }
+
+    method AddLocIfPresent(ref: BT.G.Reference, loc: BC.Location)
+    returns (added : bool)
+    requires Inv()
+    modifies Repr
+    ensures Inv()
+    ensures forall o | o in Repr :: fresh(o) || o in old(Repr)
+    ensures (I(), added) == IndirectionTableModel.AddLocIfPresent(old(I()), ref, loc)
+    {
+      IndirectionTableModel.reveal_AddLocIfPresent();
+
+      assume this.t.Count as nat < 0x10000000000000000 / 8;
+      var oldEntry := this.t.Get(ref);
+      added := oldEntry.Some? && oldEntry.value.loc.None?;
+      if added {
+        this.t.Insert(ref, IndirectionTableModel.Entry(Some(loc), oldEntry.value.succs));
+      }
+
+      Repr := {this} + this.t.Repr;
+    }
+
+    method RemoveRef(ref: BT.G.Reference)
+    returns (oldLoc : Option<BC.Location>)
+    requires Inv()
+    modifies Repr
+    ensures Inv()
+    ensures forall o | o in Repr :: fresh(o) || o in old(Repr)
+    ensures (I(), oldLoc) == IndirectionTableModel.RemoveRef(old(I()), ref)
+    {
+      IndirectionTableModel.reveal_RemoveRef();
+
+      var oldEntry := this.t.RemoveAndGet(ref);
+      oldLoc := if oldEntry.Some? then oldEntry.value.loc else None;
+
+      Repr := {this} + this.t.Repr;
+    }
+
+    method UpdateAndRemoveLoc(ref: BT.G.Reference, succs: seq<BT.G.Reference>)
+    returns (oldLoc : Option<BC.Location>)
+    requires Inv()
+    modifies Repr
+    ensures Inv()
+    ensures forall o | o in Repr :: fresh(o) || o in old(Repr)
+    ensures (I(), oldLoc)  == IndirectionTableModel.UpdateAndRemoveLoc(old(I()), ref, succs)
+    {
+      IndirectionTableModel.reveal_UpdateAndRemoveLoc();
+
+      assume this.t.Count as nat < 0x10000000000000000 / 8;
+      var oldEntry := this.t.InsertAndGetOld(ref, IndirectionTableModel.Entry(None, succs));
+      oldLoc := if oldEntry.Some? then oldEntry.value.loc else None;
+
+      Repr := {this} + this.t.Repr;
+    }
+
+    // Parsing and marshalling
+
+    static method {:fuel ValInGrammar,3} ValToHashMap(a: seq<V>) returns (s : Option<HashMap>)
+    requires IndirectionTableModel.valToHashMap.requires(a)
+    ensures s.None? ==> IndirectionTableModel.valToHashMap(a).None?
+    ensures s.Some? ==> s.value.Inv()
+    ensures s.Some? ==> Some(s.value.I()) == IndirectionTableModel.valToHashMap(a)
+    ensures s.Some? ==> s.value.Count as nat == |a|
+    ensures s.Some? ==> s.value.Count as nat < 0x1_0000_0000_0000_0000 / 8
+    ensures s.Some? ==> fresh(s.value) && fresh(s.value.Repr)
+    {
+      assume |a| < 0x1_0000_0000_0000_0000;
+      if |a| as uint64 == 0 {
+        var newHashMap := new MutableMap.ResizingHashMap<IndirectionTableModel.Entry>(1024); // TODO(alattuada) magic numbers
+        s := Some(newHashMap);
+        assume s.value.Count as nat == |a|;
+      } else {
+        var res := ValToHashMap(a[..|a| as uint64 - 1]);
+        match res {
+          case Some(mutMap) => {
+            var tuple := a[|a| as uint64 - 1];
+            var ref := tuple.t[0 as uint64].u;
+            var lba := tuple.t[1 as uint64].u;
+            var len := tuple.t[2 as uint64].u;
+            var succs := Some(tuple.t[3 as uint64].ua);
+            match succs {
+              case None => {
+                s := None;
+              }
+              case Some(succs) => {
+                var graphRef := mutMap.Get(ref);
+                var loc := LBAType.Location(lba, len);
+                if graphRef.Some? || lba == 0 || !LBAType.ValidLocation(loc) {
+                  s := None;
+                } else {
+                  mutMap.Insert(ref, IndirectionTableModel.Entry(Some(loc), succs));
+                  s := Some(mutMap);
+                  assume s.Some? ==> s.value.Count as nat < 0x10000000000000000 / 8; // TODO(alattuada) removing this results in trigger loop
+                  assume s.value.Count as nat == |a|;
+                }
+              }
+            }
+          }
+          case None => {
+            s := None;
+          }
+        }
+      }
+    }
+
+    static method GraphClosed(table: HashMap) returns (result: bool)
+      requires table.Inv()
+      requires BC.GraphClosed.requires(IndirectionTableModel.IHashMap(table.I()).graph)
+      ensures BC.GraphClosed(IndirectionTableModel.IHashMap(table.I()).graph) == result
+    {
+      var m := table.ToMap();
+      var m' := map ref | ref in m :: m[ref].succs;
+      result := BC.GraphClosed(m');
+    }
+
+    constructor(t: HashMap)
+    ensures this.t == t
+    {
+      this.t := t;
+    }
+
+    static method ValToIndirectionTable(v: V)
+    returns (s : IndirectionTable?)
+    requires IndirectionTableModel.valToIndirectionTable.requires(v)
+    ensures s != null ==> s.Inv()
+    ensures s != null ==> fresh(s.Repr)
+    ensures s == null ==> IndirectionTableModel.valToIndirectionTable(v).None?
+    ensures s != null ==> IndirectionTableModel.valToIndirectionTable(v) == Some(s.I())
+    {
+      var res := ValToHashMap(v.a);
+      match res {
+        case Some(res) => {
+          var rootRef := res.Get(BT.G.Root());
+          var isGraphClosed := GraphClosed(res);
+          if rootRef.Some? && isGraphClosed {
+            s := new IndirectionTable(res);
+            s.Repr := {s} + s.t.Repr;
+          } else {
+            s := null;
+          }
+        }
+        case None => {
+          s := null;
+        }
+      }
+    }
+
+    // To bitmap
+
+    method InitLocBitmap()
+    returns (success: bool, bm: Bitmap.Bitmap)
+    requires Inv()
+    requires BC.WFCompleteIndirectionTable(IndirectionTableModel.I(I()))
+    ensures bm.Inv()
+    ensures (success, bm.I()) == IndirectionTableModel.InitLocBitmap(old(I()))
+    ensures fresh(bm.Repr)
+    {
+      IndirectionTableModel.reveal_InitLocBitmap();
+
+      bm := new Bitmap.Bitmap(NumBlocksUint64());
+      bm.Set(0);
+      var it := t.IterStart();
+      while it.next.Some?
+      invariant t.Inv()
+      invariant BC.WFCompleteIndirectionTable(IndirectionTableModel.I(I()))
+      invariant bm.Inv()
+      invariant MutableMapModel.WFIter(t.I(), it)
+      invariant Bitmap.Len(bm.I()) == NumBlocks()
+      invariant IndirectionTableModel.InitLocBitmapIterate(I(), it, bm.I())
+             == IndirectionTableModel.InitLocBitmap(I())
+      invariant fresh(bm.Repr)
+      decreases it.decreaser
+      {
+        var kv := it.next.value;
+
+        assert kv.0 in IndirectionTableModel.I(I()).locs;
+
+        var loc: uint64 := kv.1.loc.value.addr;
+        var locIndex: uint64 := loc / BlockSizeUint64();
+        if locIndex < NumBlocksUint64() {
+          var isSet := bm.GetIsSet(locIndex);
+          if !isSet {
+            it := t.IterInc(it);
+            bm.Set(locIndex);
+          } else {
+            success := false;
+            return;
+          }
+        } else {
+          success := false;
+          return;
+        }
+      }
+
+      success := true;
+    }
+    
+    ///// Dealloc stuff
+
+    /*
+    predicate deallocable(self: IndirectionTable, ref: BT.G.Reference)
+    {
+      && ref in I(self).graph
+      && ref != BT.G.Root()
+      && (forall r | r in I(self).graph :: ref !in I(self).graph[r])
+    }
+
+    function FindDeallocableIterate(self: IndirectionTable, ephemeralRefs: seq<BT.G.Reference>, i: uint64)
+    : (ref: Option<BT.G.Reference>)
+    requires 0 <= i as int <= |ephemeralRefs|
+    requires |ephemeralRefs| < 0x1_0000_0000_0000_0000;
+    decreases 0x1_0000_0000_0000_0000 - i as int
+    {
+      if i == |ephemeralRefs| as uint64 then (
+        None
+      ) else (
+        var ref := ephemeralRefs[i];
+        var isDeallocable := deallocable(self, ref);
+        if isDeallocable then (
+          Some(ref)
+        ) else (
+          FindDeallocableIterate(self, ephemeralRefs, i + 1)
+        )
+      )
+    }
+
+    function {:opaque} FindDeallocable(self: IndirectionTable)
+    : (ref: Option<BT.G.Reference>)
+    requires Inv(self)
+    {
+      // TODO once we have an lba freelist, rewrite this to avoid extracting a `map` from `s.ephemeralIndirectionTable`
+      var ephemeralRefs := setToSeq(self.t.contents.Keys);
+
+      assume |ephemeralRefs| < 0x1_0000_0000_0000_0000;
+
+      FindDeallocableIterate(self, ephemeralRefs, 0)
+    }
+
+    lemma FindDeallocableIterateCorrect(self: IndirectionTable, ephemeralRefs: seq<BT.G.Reference>, i: uint64)
+    requires Inv(self)
+    requires 0 <= i as int <= |ephemeralRefs|
+    requires |ephemeralRefs| < 0x1_0000_0000_0000_0000;
+    requires ephemeralRefs == setToSeq(self.t.contents.Keys)
+    requires forall k : nat | k < i as nat :: (
+          && ephemeralRefs[k] in I(self).graph
+          && !deallocable(self, ephemeralRefs[k]))
+    ensures var ref := FindDeallocableIterate(self, ephemeralRefs, i);
+        && (ref.Some? ==> ref.value in I(self).graph)
+        && (ref.Some? ==> deallocable(self, ref.value))
+        && (ref.None? ==> forall r | r in I(self).graph :: !deallocable(self, r))
+    decreases 0x1_0000_0000_0000_0000 - i as int
+    {
+      if i == |ephemeralRefs| as uint64 {
+        assert forall r | r in I(self).graph :: !deallocable(self, r);
+      } else {
+        var ref := ephemeralRefs[i];
+        var isDeallocable := deallocable(self, ref);
+        if isDeallocable {
+        } else {
+          FindDeallocableIterateCorrect(self, ephemeralRefs, i + 1);
+        }
+      }
+    }
+
+    lemma FindDeallocableCorrect(self: IndirectionTable)
+    requires Inv(self)
+    ensures var ref := FindDeallocable(self);
+        && (ref.Some? ==> ref.value in I(self).graph)
+        && (ref.Some? ==> deallocable(self, ref.value))
+        && (ref.None? ==> forall r | r in I(self).graph :: !deallocable(self, r))
+    {
+      reveal_FindDeallocable();
+      var ephemeralRefs := setToSeq(self.t.contents.Keys);
+      assume |ephemeralRefs| < 0x1_0000_0000_0000_0000;
+      FindDeallocableIterateCorrect(self, ephemeralRefs, 0);
+    }
+    */
+  }
+}
